src/lib/kuiper/Kuiper.Base.fsti
@@ -6,18 +6,49 @@ open FStar.Ghost
 open Pulse.Lib.Core
 open Pulse.Main
 module SZ = Kuiper.SizeT
+module T = FStar.Tactics.V2
+val is_thread_loc (l:loc_id) : prop
+let thread_loc = l:loc_id { is_thread_loc l }
 
-type mode_t = | CPU | GPU
+val gpu_of: loc_id -> loc_id
+val gpu_of_idem (l:loc_id) : Lemma (gpu_of (gpu_of l) == l)
 
-val mode : mode_t -> slprop
+val block_of : loc_id -> loc_id
+val block_of_idem (l:loc_id) : Lemma (block_of (block_of l) == l)
 
-(* Token for being in CPU code *)
-unfold
-let cpu : slprop = mode CPU
+val gpu_id_loc (gpu_id:int) : loc_id
+
+val block_id_loc (#[T.exact (`0)]gpu_id:int) (bid:int)
+: l:loc_id { gpu_of l == gpu_id_loc gpu_id }
+
+val thread_id_loc (#[T.exact (`0)]gpu_id:int) (bid tid:int)
+: l:loc_id { block_of l == block_id_loc #gpu_id bid /\ gpu_of l == gpu_id_loc gpu_id } 
 
 (* Token for being in GPU code *)
-unfold
-let gpu : slprop = mode GPU
+[@@no_mkeys]
+let gpu (#[T.exact (`0)] gpu_id:int) : slprop =
+  exists* (l:loc_id). loc l ** pure (gpu_of l == gpu_id_loc gpu_id)
+
+(* Token given to a particular block within a grid. Both here
+and in thread_id, the first argument is always positive
+when this resource is actually live, but not placing that refinement
+here helps with inference in some places. *)
+[@@no_mkeys]
+let block_id (#[T.exact (`0)]gpu_id:int) (nblk : int) (bid : int) : slprop =
+  exists* (l:loc_id). loc l ** pure (block_of l == block_id_loc #gpu_id bid)
+
+(* Token given to a particular thread within a block *)
+[@@no_mkeys]
+let thread_id (nthr : int) (#[T.exact (`0)]gpu_id:int) (bid tid : int) : slprop =
+  loc (thread_id_loc #gpu_id bid tid)
+
+val is_cpu_loc (l:loc_id) : prop
+
+val is_cpu_loc_single_process (l0 l1:loc_id) 
+: Lemma (is_cpu_loc l0 /\ is_cpu_loc l1 ==> process_of l0 == process_of l1)
+
+(* Token for being in CPU code *)
+let cpu : slprop = exists* l. loc l ** pure (is_cpu_loc l)
 
 (* Token allowing to create a barrier for n threads. Only
    available while in the block_setup of a kernel. *)
@@ -58,16 +89,6 @@ unfold let warp_sz = 32sz
 inline_for_extraction noextract
 unfold let warp_size = 32
 
-(* Token given to a particular block within a grid. Both here
-and in thread_id, the first argument is always positive
-when this resource is actually live, but not placing that refinement
-here helps with inference in some places. *)
-[@@no_mkeys]
-val block_id (nblk : int) (bid : int) : slprop
-
-(* Token given to a particular thread within a block *)
-[@@no_mkeys]
-val thread_id (nthr : int) (tid : int) : slprop
 
 (* Get a concrete value for the number of blocks (~ gridDim.x) *)
 fn get_gdim ()
@@ -77,6 +98,6 @@ fn get_gdim ()
 
 (* Get a concrete value for the number of threads (~ blockDim.x) *)
 fn get_bdim ()
-  preserves thread_id 'nthr 'tid
+  preserves thread_id 'nthr 'bid 'tid
   returns   x : SZ.t
   ensures   pure (SZ.v x == 'nthr)
